axiom elem_context_det tweaking, some refactoring

refocusing_signatures.v
@@ -14,33 +14,34 @@ Module Type RED_SEM (R : RED_LANG).
 
   Axiom decompose : forall (t : term) k1, ~ dead_ckind k1 ->
       (exists (v : value k1), t = v) \/
-      (exists k2 (r : redex k2) (c : context k1 k2), c[r] = t).
+      (exists k2 (r : redex k2) (c : context k1 k2), t = c[r]).
 
   (** dec is left inverse of plug *)
-  Axiom dec_correct  : forall t {k1 k2} (c : context k1 k2) d, dec t c d -> 
-                           decomp_to_term d = c[t].
+  Axiom dec_correct  : forall {t k1 k2} {c : context k1 k2} {d}, 
+                           dec t c d -> c[t] = d.
 
-  Axiom dec_plug     : forall {k1 k2} (c : context k1 k2) {k3} (c0 : context k3 k1) t d, 
+  Axiom dec_plug     : forall {k1 k2} (c : context k1 k2) {k3} {c0 : context k3 k1} {t d}, 
                            ~ dead_ckind k2 -> dec c[t] c0 d -> 
                            dec t (c ~+ c0) d.
 
-  Axiom dec_plug_rev : forall {k1 k2} (c : context k1 k2) {k3} (c0 : context k3 k1) t d, 
+  Axiom dec_plug_rev : forall {k1 k2} (c : context k1 k2) {k3} {c0 : context k3 k1} {t d}, 
                            ~ dead_ckind k2 ->  dec t (c ~+ c0) d -> 
                            dec c[t] c0 d.
 
   Inductive decempty : term -> forall {k}, decomp k -> Prop :=
-  | d_intro : forall t {k} (d : decomp k), dec t [_] d -> decempty t d.
+  | d_intro : forall {t k} {d : decomp k}, dec t [_] d -> decempty t d.
 
   Inductive iter : forall {k}, decomp k -> value k -> Prop :=
   | i_val : forall {k} (v : value k), iter (d_val v) v
-  | i_red : forall {k2} (r : redex k2) t {k1} (c : context k1 k2) d v,
+  | i_red : forall {k2} (r : redex k2) {t k1} (c : context k1 k2) {d v},
               contract r = Some t -> decempty c[t] d -> iter d v ->
               iter (d_red r c) v.
 
   Inductive eval : term -> forall {k}, value k -> Prop :=
-  | e_intro : forall t {k} (d : decomp k) v, decempty t d -> iter d v -> eval t v.
+  | e_intro : forall {t k} {d : decomp k} {v}, decempty t d -> iter d v -> eval t v.
 
 End RED_SEM.
+
 
 
 Module Type RED_REF_SEM (R : RED_LANG).
@@ -52,36 +53,33 @@ Module Type RED_REF_SEM (R : RED_LANG).
   Parameter dec_context : forall ec k, value (k+>ec) -> interm_dec k.
 
 
-  (*Axiom dec_term_liveness : 
-      forall t k, ~ dead_ckind k -> 
-      forall t0 ec0, dec_term t k = in_term t0 ec0 ->
-      ~ dead_ckind (ckind_trans k ec0).*)
+  Axiom dec_term_correct : 
+      forall t k, match dec_term t k with
+      | in_red r       => t = r
+      | in_val v       => t = v
+      | in_term t0 ec0 => t = ec0:[t0]
+      | in_dead        => dead_ckind k
+      end.
 
-  Axiom dec_term_correct : forall t k, match dec_term t k with
-    | in_red r       => t = r
-    | in_val v       => t = v
-    | in_term t0 ec0 => t = ec0:[t0]
-    | in_dead        => dead_ckind k
-  end.
-
-  Axiom dec_context_correct : forall ec k v, match dec_context ec k v with
-    | in_red r      => ec:[v] = r
-    | in_val v0     => ec:[v] = v0
-    | in_term t ec0 => ec:[v] = ec0:[t]
-    | in_dead       => dead_ckind (k+>ec) 
-  end.
+  Axiom dec_context_correct : 
+      forall ec k v, match dec_context ec k v with
+      | in_red r      => ec:[v] = r
+      | in_val v0     => ec:[v] = v0
+      | in_term t ec0 => ec:[v] = ec0:[t]
+      | in_dead       => dead_ckind (k+>ec) 
+      end.
 
 
   (** A decomposition function specified in terms of the atomic functions above *)
   Inductive dec : term -> forall {k1 k2}, context k1 k2 -> decomp k1 -> Prop :=
-  | d_dec  : forall t {k1 k2} (c : context k1 k2) r,
+  | d_dec  : forall t {k1 k2} (c : context k1 k2) {r},
                dec_term t k2 = in_red r -> 
                dec t c (d_red r c)
-  | d_v    : forall t {k1 k2} (c : context k1 k2) v d,
+  | d_v    : forall t {k1 k2} {c : context k1 k2} {v d},
                dec_term t k2 = in_val v ->
                decctx v c d ->
                dec t c d
-  | d_term : forall t t0 {k1 k2} (c : context k1 k2) ec d,
+  | d_term : forall t {t0 k1 k2} {c : context k1 k2} {ec d},
                dec_term t k2 = in_term t0 ec ->
                dec t0 (ec=:c) d ->
                dec t c d
@@ -89,16 +87,16 @@ Module Type RED_REF_SEM (R : RED_LANG).
   | dc_end  : forall {k} (v : value k), 
                 ~ dead_ckind k ->
                 decctx v [_] (d_val v)
-  | dc_dec  : forall ec {k2} (v : value (k2+>ec)) {k1} (c : context k1 k2) r,
+  | dc_dec  : forall ec {k2} (v : value (k2+>ec)) {k1} (c : context k1 k2) {r},
                 dec_context ec k2 v = in_red r ->
                 decctx v (ec=:c) (d_red r c)
-  | dc_val  : forall {k2} (v0 : value k2) ec (v : value (k2+>ec)) 
-                     {k1} (c  : context k1 k2) d,
+  | dc_val  : forall {k2} {v0 : value k2} ec (v : value (k2+>ec)) 
+                     {k1} {c  : context k1 k2} {d},
                 dec_context ec k2 v = in_val v0 ->
                 decctx v0 c d ->
                 decctx v (ec=:c) d
-  | dc_term : forall ec ec0 {k2} (v : value (k2+>ec)) 
-                            {k1} (c : context k1 k2) t d,
+  | dc_term : forall ec {ec0 k2} (v : value (k2+>ec)) 
+                            {k1} {c : context k1 k2} {t d},
                 dec_context ec k2 v = in_term t ec0 ->
                 dec t (ec0=:c) d ->
                 decctx v (ec=:c) d.
@@ -107,8 +105,8 @@ Module Type RED_REF_SEM (R : RED_LANG).
    with decctx_Ind := Induction for decctx Sort Prop.
 
 
-  Axiom dec_val_self : forall {k2} (v : value k2) {k1} (c : context k1 k2) d, 
-                           dec (value_to_term v) c d <-> decctx v c d.
+  Axiom dec_val_self : forall {k2} (v : value k2) {k1} {c : context k1 k2} {d}, 
+                           dec v c d <-> decctx v c d.
 
   Declare Module RS : RED_SEM R with Definition dec := dec.
 
@@ -134,24 +132,24 @@ Module Type RED_SEM_PROPER (R : RED_LANG) (RS : RED_SEM R).
   Import R.
   Import RS.
 
-  Axiom dec_is_function  : forall t {k} (d d0 : decomp k), 
+  Axiom dec_is_function  : forall {t k} {d d0 : decomp k}, 
                                decempty t d -> decempty t d0 -> d = d0.
-  Axiom iter_is_function : forall {k} (d : decomp k) v v0, 
+  Axiom iter_is_function : forall {k} {d : decomp k} {v v0}, 
                                iter d v -> iter d v0 -> v = v0.
-  Axiom eval_is_function : forall t {k} (v v0 : value k), 
+  Axiom eval_is_function : forall {t k} {v v0 : value k}, 
                                eval t v -> eval t v0 -> v = v0.
-  Axiom dec_correct      : forall t {k1 k2} (c : context k1 k2) d,
+  Axiom dec_correct      : forall {t k1 k2} {c : context k1 k2} {d},
                                dec t c d -> decomp_to_term d = plug t c.
   Axiom dec_total        : forall t k, ~ dead_ckind k -> 
                                exists (d : decomp k), decempty t d.
-  Axiom unique_decomposition : 
+  Axiom unique_decomposition :
 
-      forall t k1, ~ dead_ckind k1 ->  
+      forall (t : term) k1, ~ dead_ckind k1 ->  
 
-         (exists v : R.value k1, value_to_term v = t) \/
+         (exists v : value k1, t = v) \/
 
-         (exists k2 (r : redex k2) (c : context k1 k2), c[r] = t /\ 
+         (exists k2 (r : redex k2) (c : context k1 k2), t = c[r] /\ 
 	      forall k2' (r' : redex k2') (c' : context k1 k2'), 
-                  c'[r'] = t -> k2' = k2 /\ r ~= r' /\ c ~= c').
+                  t = c'[r'] -> k2' = k2 /\ r ~= r' /\ c ~= c').
 
 End RED_SEM_PROPER.
